---
marp: true
theme: uncover
class: invert
paginate: true
math: mathjax
---

# <!--fit--> Pre-Calculus 11 Notes
<span style="color:grey">By:</span> Gen L.

<!--_footer: In partnership with Hyperion University, 2023-->

$\newcommand{\wfr}[1]{\frac{#1}{1}}$

---

## Lesson 4: Rational Equations

---

## Steps

1) NPVs
2) Common Denominator
3) Cut the Denominator
4) Solve

---

## Example 1

1) $\frac{3x}{4}=\frac{2x}{3}-\frac{3}{2}$
    * NPVs: None, LCD: 12
2) $3(\frac{3x}{4})=4(\frac{2x}{3})-6(\frac{3}{2})$
    * Simplify & Cut
3) $9x=8x-18$
    * Solve
4) $x=-18$

---

## Example 2

1) $\frac{x}{4}-\frac{7}{x}=\wfr{3}$
    * NPVs: $x\neq0$ & LCD: $4x$
2) $x(\frac{x}{4})-4(\frac{7}{x})=4x(\wfr{3})$
    * Simplify & Cut
3) $x^2-28=12x$
    * Solve
4) $x^2-12x-28=0$
    * Factor
5) $(x-14)(x+2)$
    * Set to 0: $x=14,-2$

---

## Example 3

1) $\frac{9}{y-3}-\frac{4}{y-6}=\frac{18}{y^2-9y+18}$
    * Factor
2) $\frac{9}{y-3}-\frac{4}{y-6}=\frac{18}{(y-6)(y-3)}$
    * NPVs: $y\neq3,6$ & LCD: $(y-3)(y-6)$
3) $(y-6)(\frac{9}{y-3})-(y-3)(\frac{4}{y-6})=\frac{18}{(y-6)(y-3)}$
    * Simplify & Cut
4) $9(y-6)-4(y-3)=18$
    * Solve
5) $5y-42=18$
    * $y=12$

---

## Example 4

1) $\frac{4k-1}{k+2}-\frac{k+1}{k-2}=\frac{k^2-4k+24}{k^2-4}$
    * Factor
2) $\frac{4k-1}{k+2}-\frac{k+1}{k-2}=\frac{k^2-4k+24}{(k+2)(k-2)}$
    * NPVs: $k\neq\pm2$ & LCD: $(k+2)(k-2)$
3) $(k-2)(\frac{4k-1}{k+2})-(k+2)\frac{k+1}{k-2}=\frac{k^2-4k+24}{(k+2)(k-2)}$
    * Simplify & Cut
4) $4k^2-9k+2-k^2+3k+2=k^2-4k+24$
    * $2k^2-8k+24=0$
    * $2(k-6)(k+2)$
    * $k=6$

